WIP; pg, core, helpee cases left

helping/HelpingOn.v
@@ -29,16 +29,16 @@ Section HoareCall.
     | None => unit
     end.
 
-  Definition HoareCall_prologue fspo parg : itree crisE (fspec_option_meta fspo * Any.t) :=
+  Definition HoareCall_prologue fspo varg : itree crisE (fspec_option_meta fspo * Any.t) :=
     Seal.sealing "Help"
     (match fspo as fspo return itree crisE (fspec_option_meta fspo * Any.t) with
     | Some (@fspec_call _ meta pre post) =>
         x <- trigger (Choose meta);;
-        varg <- trigger (Choose Any.t);;
-        trigger (Guarantee (pre x parg varg));;;
-        Ret (x, varg)
+        arg <- trigger (Choose Any.t);;
+        trigger (Guarantee (pre x varg arg));;;
+        Ret (x, arg)
     | Some _ => triggerNB
-    | None => Ret (tt, parg)
+    | None => Ret (tt, varg)
     end).
 
   Definition HoareCall_epilogue fspo (x : fspec_option_meta fspo) (pret : Any.t)
@@ -67,11 +67,36 @@ Section HoareCall.
     { ired. f_equal. extensionalities; ss. }
     { ired. erewrite <-bind_ret_r at 1. f_equal. extensionalities a. unseal "Help". done. }
   Qed.
+
+  Definition HoareFun_prologue fspo parg : itree crisE (fspec_option_meta fspo * Any.t) :=
+    Seal.sealing "Help"
+    (match fspo as fspo return itree crisE (fspec_option_meta fspo * Any.t) with
+    | Some (@fspec_call _ meta pre post) =>
+        x <- trigger (Take meta);;
+        varg <- trigger (Take Any.t);;
+        trigger (Assume (post x varg parg));;;
+        Ret (x, varg)
+    | Some _ => triggerNB
+    | None => Ret (tt, parg)
+    end).
+
+  Definition HoareFun_epilogue fspo (x : fspec_option_meta fspo) (vret : Any.t)
+      : itree crisE Any.t :=
+    Seal.sealing "Help"
+    (match fspo as fspo return fspec_option_meta fspo → itree crisE Any.t with
+    | Some (@fspec_call _ meta pre post) =>
+        λ x,
+          pret <- trigger (Choose Any.t);;
+          trigger (Guarantee (pre x vret pret));;;
+          Ret pret
+    | Some _ => λ _, triggerNB
+    | None => λ _, Ret vret
+    end) x.
 End HoareCall.
 
 (* Helping module *)
 Module HelpingOn. Section HelpingOn.
-  Context `{!crisG Γ Σ α β τ _S _I, !concG} {jobID : Type}.
+  Context `{!crisG Γ Σ α β τ _S _I, !concG} `{LeibnizEquiv jobID}.
 
   Context (mn : string).
   Context (jobcode : jobID → itree Helping.pureE unit).
@@ -95,16 +120,16 @@ Module HelpingOn. Section HelpingOn.
       'reqs : gmap nat jobID <- cgetU v_reqs;;
       let tid := fresh (dom reqs) in
       cput v_reqs (<[tid := jid]> reqs);;;
-      𝒴;;;
-      try_run tid.
+      𝒴;;; try_run tid;;; 𝒴;;; Ret ()↑.
 
   Definition help (sp : sp_type) : Any.t → itree crisE Any.t :=
     λ _,
       tid <- trigger (Choose nat);;
       xarg <- HoareCall_prologue (sp SchHdr.yield) (() ↑);;
-      HoareCall_epilogue (sp SchHdr.yield) xarg.1 (() ↑);;;
+      x <- HoareFun_prologue (sp SchHdr.yield) (() ↑);;
       try_run tid;;;
-      𝒴;;;
+      HoareFun_epilogue (sp SchHdr.yield) x.1 (() ↑);;;
+      HoareCall_epilogue (sp SchHdr.yield) xarg.1 (() ↑);;;
       Ret ()↑.
 
   Definition fnsems (sp : sp_type) : alist (option string) (fnsem_type (option fspec * fbody)) :=
